Prove a whole_prog_thm-style thm for cyes

examples/cost/cyesProgScript.sml
@@ -55,9 +55,10 @@ val _ = (append_prog o process_topdecs) `
   fun printLoop c = (put_char c; printLoop c);
   `
 
+val maincall = process_topdecs `val _ = printLoop #"a"`
+
 local
   val prog = get_prog(get_ml_prog_state())
-  val maincall = process_topdecs `val _ = printLoop #"a"`
 in
   val cyes = (rhs o concl o EVAL) ``^prog ++ ^maincall``
 end
@@ -74,7 +75,7 @@ val put_str_event_def = Define `
   put_str_event cs = IO_event "put_char" (MAP (n2w o ORD) cs) []`;
 
 val update_def = Define `
-  (update "put_char" cs [] s = SOME (FFIreturn [] s))`
+  (update "put_char" cs l s = SOME (FFIreturn l s))`
 
 val State_def = Define `
   State = Stream [||]`
@@ -263,6 +264,207 @@ Proof
     \\ MAP_EVERY qexists_tac [`emp`, `[]`, `c`]
     \\ xsimpl)
   \\ xvar \\ xsimpl
+QED
+
+val sio_oracle = Define `
+  (sio_oracle:unit oracle) port st conf bytes =
+  if port = "put_char" then
+    Oracle_return st bytes
+  else Oracle_final FFI_failed
+`
+
+val encode_oracle_state_def = Define `
+  encode_oracle_state(st:unit) =
+      State`
+
+val decode_oracle_state_def = Define `
+  decode_oracle_state(st:ffi) = ()`
+
+Theorem decode_encode_oracle_state_11:
+  !ffi_st. decode_oracle_state(encode_oracle_state ffi_st) = ffi_st
+Proof
+  rw[encode_oracle_state_def,decode_oracle_state_def]
+QED
+
+val sio_proj1_def = Define `
+  sio_proj1 = (λffi.
+    FEMPTY |++ (mk_proj1 (encode_oracle_state,decode_oracle_state,
+                          [("put_char", sio_oracle "put_char")]) ffi))`;
+
+val sio_proj2 = Define `sio_proj2 =
+  [(["put_char"],update)]`
+
+Theorem limited_parts_proj:
+  limited_parts ["put_char"] (sio_proj1,sio_proj2)
+Proof
+  rw[limited_parts_def,sio_proj2]
+QED
+
+val sio_ffi_state_def = Define `sio_ffi_state =
+  <|oracle:=sio_oracle; ffi_state := (); io_events := []|>`;
+
+Theorem parts_ok_filter:
+  parts_ok sio_ffi_state (sio_proj1,sio_proj2)
+Proof
+  rw[cfStoreTheory.parts_ok_def,sio_proj1_def,sio_proj2,sio_ffi_state_def,
+     cfStoreTheory.ffi_has_index_in_def,mk_proj1_def,FLOOKUP_UPDATE,
+     FUPDATE_LIST_THM,FAPPLY_FUPDATE_THM,decode_encode_oracle_state_11,
+     sio_oracle,update_def]
+QED
+
+Theorem semantics_prog_thm:
+ semantics_prog ((^(get_state st)) with ffi:= sio_ffi_state) ^(get_env st)
+  (^maincall)
+  (Diverge(LREPEAT [put_char_event #"a"]))
+Proof
+  rpt strip_tac >>
+  `nsLookup ^(get_env st).v (Short "printLoop") = SOME printLoop_v`
+    by(unabbrev_all_tac >> EVAL_TAC) >>
+  assume_tac limited_parts_proj >>
+  FULL_SIMP_TAC bool_ss [GSYM names_def] >>
+  drule printLoop_spec >>
+  disch_then(qspec_then `#"a"` mp_tac) >>
+  disch_then(qspec_then `Litv(Char #"a")` mp_tac) >>
+  simp[app_def,app_basic_def] >>
+  disch_then(mp_tac o CONV_RULE(RESORT_FORALL_CONV rev)) >>
+  qmatch_goalsub_abbrev_tac `semantics_prog st` >>
+  disch_then(qspec_then `st` mp_tac) >>
+  unabbrev_all_tac >>
+  simp[cfStoreTheory.st2heap_def,cfStoreTheory.store2heap_append,cfStoreTheory.ffi2heap_def,
+       miniBasisProg_st_def,parts_ok_filter] >>
+  qmatch_goalsub_abbrev_tac `FFI_split INSERT FFIset` >>
+  `FFIset = {FFI_part (encode_oracle_state ()) update
+                      ["put_char"] []}`
+    by(unabbrev_all_tac >> rw[FUN_EQ_THM,EQ_IMP_THM] >-
+        (pairarg_tac >> fs[sio_proj2] >> rveq >>
+         fs[] >>
+         fs[sio_proj1_def,mk_proj1_def] >>
+         fs[FLOOKUP_UPDATE,FUPDATE_LIST_THM,sio_ffi_state_def]) >>
+       Q.REFINE_EXISTS_TAC `(s,u,ns,ts)` >>
+       rw[sio_proj2,sio_ffi_state_def,sio_proj1_def,mk_proj1_def,
+          FLOOKUP_UPDATE,FUPDATE_LIST_THM]) >>
+  simp[] >> pop_assum kall_tac >> unabbrev_all_tac >>
+  qmatch_goalsub_abbrev_tac `junk ∪ {_;FFIpart}` >>
+  disch_then(qspecl_then [`FFI_split INSERT junk`,
+                          `{FFIpart}`]
+                         mp_tac) >>
+  impl_tac >-
+    (rw[SPLIT_def] >> unabbrev_all_tac >> simp[] >-
+       (rw[FUN_EQ_THM,EQ_IMP_THM] >> rw[]) >-
+       (simp[cfStoreTheory.FFI_part_NOT_IN_store2heap_aux,
+             cfStoreTheory.store2heap_def])
+    ) >>
+  impl_tac >- (simp[SIO_def,Abbr `FFIpart`,one_def,encode_oracle_state_def,names_def]) >>
+  strip_tac >>
+  Cases_on `r` >> fs[cond_def] >> rveq >>
+  fs[evaluate_to_heap_def,semanticsTheory.semantics_prog_def] >>
+  rpt strip_tac >-
+    (simp[semanticsTheory.evaluate_prog_with_clock_def,
+          terminationTheory.evaluate_decs_def,
+          astTheory.pat_bindings_def] >>
+     simp[terminationTheory.evaluate_def] >>
+     simp[semanticPrimitivesTheory.do_con_check_def,semanticPrimitivesTheory.build_conv_def] >>
+     rw[evaluateTheory.dec_clock_def] >>
+     fs[evaluate_ck_def] >>
+     first_x_assum(qspec_then `k - 1` strip_assume_tac) >>
+     fs[]) >>
+  fs[] >>
+  match_mp_tac(GEN_ALL lprefix_lub_subset) >>
+  goal_assum drule >> simp[] >> conj_tac >-
+    (rw[IMAGE_DEF,SUBSET_DEF] >>
+     qexists_tac `SUC ck` >>
+     simp[semanticsTheory.evaluate_prog_with_clock_def,
+          terminationTheory.evaluate_decs_def,
+          astTheory.pat_bindings_def
+         ] >>
+     simp[terminationTheory.evaluate_def] >>
+     simp[semanticPrimitivesTheory.do_con_check_def,semanticPrimitivesTheory.build_conv_def] >>
+     rw[evaluateTheory.dec_clock_def] >>
+     fs[evaluate_ck_def] >>
+     rpt(PURE_TOP_CASE_TAC >> rveq >> fs[])) >>
+  rw[PULL_EXISTS] >>
+  simp[LPREFIX_fromList_fromList] >>
+  simp[semanticsTheory.evaluate_prog_with_clock_def,
+       terminationTheory.evaluate_decs_def,
+       astTheory.pat_bindings_def
+      ] >>
+  simp[terminationTheory.evaluate_def] >>
+  simp[semanticPrimitivesTheory.do_con_check_def,semanticPrimitivesTheory.build_conv_def] >>
+  rw[evaluateTheory.dec_clock_def] >>
+  fs[evaluate_ck_def] >>
+  first_x_assum(qspec_then `k - 1` strip_assume_tac) >>
+  fs[] >-
+    (qexists_tac `ARB` >>
+     qmatch_goalsub_abbrev_tac `evaluate st` >>
+     Q.ISPEC_THEN `st` mp_tac
+       (CONJUNCT1 evaluatePropsTheory.evaluate_io_events_mono
+        |> SIMP_RULE std_ss [evaluatePropsTheory.io_events_mono_def]) >>
+     simp[Abbr `st`]) >>
+  qexists_tac `k - 1` >>
+  every_case_tac >> fs[]
+QED
+
+(* TODO: this proof is slow and also an abomination. We should really make proper
+   whole_prog_thm automation for Diverge.
+ *)
+Theorem cyes_semantics_prog_Diverge:
+  let (s,env) = THE (prim_sem_env sio_ffi_state)
+  in semantics_prog s env cyes_prog (Diverge (LREPEAT [put_char_event #"a"]))
+Proof
+  rw[] >>
+  mp_tac semantics_prog_thm >>
+  disch_then (mp_tac o CONV_RULE((RATOR_CONV o RATOR_CONV o RAND_CONV) EVAL)) >>
+  disch_then (mp_tac o CONV_RULE((RATOR_CONV o RATOR_CONV o RATOR_CONV o RAND_CONV) EVAL)) >>
+  CONV_TAC(RAND_CONV(RAND_CONV(RAND_CONV EVAL))) >>
+  fs[cyes_prog_def,ml_progTheory.init_env_def] >>
+  (* TODO: can we avoid referring explicitly to these generated env defs in a cleaner way? *)
+  FULL_SIMP_TAC std_ss
+    (case st of ML_code (sts,envs,vs,_) => sts @ envs @ vs) >>
+  qabbrev_tac `maincall = ^maincall` >>
+  fs[semanticsTheory.semantics_prog_def,semanticsTheory.evaluate_prog_with_clock_def,
+     terminationTheory.evaluate_def,terminationTheory.evaluate_decs_def,
+     semanticPrimitivesTheory.check_dup_ctors_def,
+     astTheory.pat_bindings_def,
+     semanticPrimitivesTheory.combine_dec_result_def,
+     terminationTheory.pmatch_def,
+     semanticPrimitivesTheory.extend_dec_env_def,
+     semanticPrimitivesTheory.build_tdefs_def,
+     semanticPrimitivesTheory.build_constrs_def,
+     evaluatePropsTheory.evaluate_decs_cons,
+     ml_progTheory.write_def,
+     ml_progTheory.write_mod_def,
+     ml_progTheory.write_cons_def
+    ] >>
+  qmatch_goalsub_abbrev_tac `aa1  /\ aa2 ==> ab1 /\ ab2` >>
+  qsuff_tac `(aa1 = ab1) /\ (aa2 = ab2)` >-
+    (rpt(pop_assum kall_tac) >> metis_tac[]) >>
+  conj_tac >-
+    (unabbrev_all_tac >>
+     CHANGED_TAC(rpt(AP_THM_TAC ORELSE AP_TERM_TAC)) >>
+     rw[FUN_EQ_THM,ELIM_UNCURRY] >>
+     qmatch_goalsub_abbrev_tac `evaluate_decs a1 a2` >>
+     qpat_abbrev_tac `aa1 = evaluate_decs a1 a2` >>
+     qmatch_goalsub_abbrev_tac `evaluate_decs a3 a4` >>
+     `a1 = a3`
+       by(unabbrev_all_tac >> simp[semanticPrimitivesTheory.state_component_equality]) >>
+     `a2 = a4`
+       by(unabbrev_all_tac >> EVAL_TAC) >>
+     simp[Abbr `aa1`] >>
+     Cases_on `evaluate_decs a3 a4 ^maincall` >> rw[] >>
+     rw[CaseEq"semanticPrimitives$result",CaseEq"prod"]) >>
+  unabbrev_all_tac >>
+  CHANGED_TAC(rpt(AP_THM_TAC ORELSE AP_TERM_TAC)) >>
+  rw[FUN_EQ_THM,ELIM_UNCURRY] >>
+  qmatch_goalsub_abbrev_tac `evaluate_decs a1 a2` >>
+  qpat_abbrev_tac `aa1 = evaluate_decs a1 a2` >>
+  qmatch_goalsub_abbrev_tac `evaluate_decs a3 a4` >>
+  `a1 = a3`
+    by(unabbrev_all_tac >> simp[semanticPrimitivesTheory.state_component_equality]) >>
+  `a2 = a4`
+    by(unabbrev_all_tac >> EVAL_TAC) >>
+  simp[Abbr `aa1`] >>
+  Cases_on `evaluate_decs a3 a4 ^maincall` >> rw[] >>
+  rw[CaseEq"semanticPrimitives$result",CaseEq"prod"]
 QED
 
 val cyes2 =
@@ -999,11 +1201,11 @@ Theorem cyes_s_def = mk_abbrev"cyes_s"
                       ((rand o rand o rhs o concl) primSemEnvTheory.prim_sem_env_eq)
 
 Definition cyes_env_def:
-  cyes_env ffi = FST (THE (prim_sem_env ffi))
+  cyes_env ffi = FST (THE (prim_sem_env sio_ffi_state))
 End
 
 Theorem prim_sem_env_cyes:
-  THE (prim_sem_env ffi) = (cyes_env ffi,cyes_s)
+  THE (prim_sem_env sio_ffi_state) = (cyes_env ffi,cyes_s)
 Proof
 EVAL_TAC \\ rw [cyes_s_def]
 QED
@@ -1015,23 +1217,16 @@ Proof
  cheat
 QED
 
-(* TODO *)
-Theorem cyes_semantics_prog_Diverge:
-  let (s,env) = THE (prim_sem_env ffi)
-  in semantics_prog s env cyes_prog (Diverge ARB)
-Proof
-  cheat
-QED
-
 Theorem cyes_semantics_prog_Diverge_ex:
-  let (s,env) = THE (prim_sem_env ffi)
+  let (s,env) = THE (prim_sem_env sio_ffi_state)
   in ∃io_trace. semantics_prog s env cyes_prog (Diverge io_trace)
 Proof
-  cheat
+  mp_tac cyes_semantics_prog_Diverge >>
+  rw[ELIM_UNCURRY] >> goal_assum drule
 QED
 
 Theorem cyes_semantics_prog_not_Fail:
-  let (s,env) = THE (prim_sem_env ffi)
+  let (s,env) = THE (prim_sem_env sio_ffi_state)
   in ¬semantics_prog s env cyes_prog Fail
 Proof
   (* assume_tac cyes_semantics_prog_Diverge *)
